GrowImpl currently has timeout issue

Impl/GrowImpl.i.dfy
@@ -25,62 +25,62 @@ module GrowImpl {
   import opened NativeTypes
 
   /// The root was found to be too big: grow
-  method grow(s: ImplVariables)
-  requires Inv(s)
-  requires s.ready
-  requires BT.G.Root() in s.cache.I()
-  requires |s.ephemeralIndirectionTable.I().graph| <= IT.MaxSize() - 2
-  modifies s.Repr()
-  ensures WellUpdated(s)
+  method grow(linear inout s: ImplVariables)
+  requires old_s.Inv()
+  requires old_s.ready
+  requires BT.G.Root() in old_s.I().cache
+  requires |old_s.I().ephemeralIndirectionTable.graph| <= IT.MaxSize() - 2
+  ensures s.W()
   ensures s.ready
-  ensures s.I() == GrowModel.grow(old(s.I()))
+  ensures s.I() == GrowModel.grow(old_s.I())
   {
     GrowModel.reveal_grow();
 
-    BookkeepingModel.lemmaChildrenConditionsOfNode(s.I(), BT.G.Root());
+    var root := BT.G.Root();
+    BookkeepingModel.lemmaChildrenConditionsOfNode(s.I(), root);
+    var nop := false;
 
-    assert s.blockAllocator.Repr <= s.Repr();
-
-    if s.frozenIndirectionTable != null {
-      var b := s.frozenIndirectionTable.HasEmptyLoc(BT.G.Root());
+    if s.frozenIndirectionTable.lSome? {
+      var b := s.frozenIndirectionTable.value.HasEmptyLoc(root);
       if b {
         print "giving up; grow can't run because frozen isn't written";
-        return;
+        nop := true;
       }
     }
 
-    var oldpivots, oldchildren := s.cache.GetNodeInfo(BT.G.Root());
-    var containsall := ComputeContainsAllKeys(oldpivots);
-    if !containsall {
-      print "giving up; grow can't run because root node is incorrect";
-      return;
-    }
+    if !nop {
+      var oldpivots, oldchildren := s.cache.GetNodeInfo(root);
+      var containsall := ComputeContainsAllKeys(oldpivots);
+      if !containsall {
+        print "giving up; grow can't run because root node is incorrect";
+      } else {
+        BookkeepingModel.lemmaChildrenConditionsSingleOfAllocBookkeeping(s.I(), oldchildren);
+        var newref := allocBookkeeping(inout s, oldchildren);
+        match newref {
+          case None => {
+            print "giving up; could not allocate ref\n";
+          }
+          case Some(newref) => {
+            WeightBucketEmpty();
 
-    BookkeepingModel.lemmaChildrenConditionsSingleOfAllocBookkeeping(s.I(), oldchildren);
-    var newref := allocBookkeeping(s, oldchildren);
-    match newref {
-      case None => {
-        print "giving up; could not allocate ref\n";
-      }
-      case Some(newref) => {
-        WeightBucketEmpty();
+            linear var mutbucket := MutBucket.Alloc();
+            linear var buckets := lseq_alloc(1);
+            lseq_give_inout(inout buckets, 0, mutbucket);
 
-        linear var mutbucket := MutBucket.Alloc();
-        linear var buckets := lseq_alloc(1);
-        lseq_give_inout(inout buckets, 0, mutbucket);
+            linear var newroot := Node(InitPivotTable(), Some([newref]), buckets);
+            assert newroot.I() == BT.G.Node(InitPivotTable(), Some([newref]), [B(map[])]);
+            assert s.I().cache[root] == old_s.I().cache[root];
 
-        linear var newroot := Node(InitPivotTable(), Some([newref]), buckets);
-        assert newroot.I() == BT.G.Node(InitPivotTable(), Some([newref]), [B(map[])]);
-        assert s.I().cache[BT.G.Root()] == old(s.I().cache[BT.G.Root()]);
+            writeBookkeeping(inout s, root, Some([newref]));
+            inout s.cache.MoveAndReplace(root, newref, newroot);
 
-        writeBookkeeping(s, BT.G.Root(), Some([newref]));
-        s.cache.MoveAndReplace(BT.G.Root(), newref, newroot);
-
-        ghost var a := s.I();
-        ghost var b := GrowModel.grow(old(s.I()));
-        assert a.cache == b.cache;
-        assert a.ephemeralIndirectionTable == b.ephemeralIndirectionTable;
-        assert a.lru == b.lru;
+            ghost var a := s.I();
+            ghost var b := GrowModel.grow(old_s.I());
+            assert a.cache == b.cache;
+            assert a.ephemeralIndirectionTable == b.ephemeralIndirectionTable;
+            assert a.lru == b.lru;
+          }
+        }
       }
     }
   }
